src/theories/FOLTrees.v
@@ -1,0 +1,170 @@
+From Equations Require Import Equations.
+Require Import Coq.Program.Equality.
+Require Import Coq.Lists.List.
+
+Require Import MirrorSolve.FirstOrder.
+Require Import MirrorSolve.HLists.
+
+Import ListNotations.
+Import HListNotations.
+
+Set Universe Polymorphism.
+
+Require Import Coq.ZArith.BinInt.
+
+Section Tree.
+  (* type of values in the tree *)
+  Variable (V: Type).
+
+  Inductive tree :=
+    | Emp
+    | Node (l : tree) (k : Z) (v : V) (r : tree).
+
+(** [bound k t] is whether [k] is bound in [t]. *)
+
+  Fixpoint bound (x : Z) (t : tree) :=
+    match t with
+    | Emp => false
+    | Node l y v r => 
+      ite (x <? y)%Z (bound x l)
+      (ite (x >? y)%Z (bound x r) true)
+    end.
+
+  Lemma bound_emp: 
+    forall x, 
+      bound x Emp = false.
+  Proof. intros; exact eq_refl. Qed.
+
+  Lemma bound_node: 
+    forall x l y v r, 
+      bound x (Node l y v r) = ( 
+        ite (x <? y)%Z (bound x l)
+        (ite (x >? y)%Z (bound x r) true)
+      ).
+  Proof. intros; exact eq_refl. Qed.
+
+  (** [lookup d k t] is the value bound to [k] in [t], or is default
+      value [d] if [k] is not bound in [t]. *)
+
+  Fixpoint lookup (d : V) (x : Z) (t : tree) : V :=
+    match t with
+    | Emp => d
+    | Node l y v r => 
+      ite (x <? y)%Z (lookup d x l)
+      (ite (x >? y)%Z (lookup d x r) v)
+    end.
+
+  Lemma lookup_emp: 
+    forall d x, 
+      lookup d x Emp = d.
+  Proof. intros; exact eq_refl. Qed.
+
+  Lemma lookup_node: 
+    forall d x l y v r, 
+      lookup d x (Node l y v r) = ( 
+        ite (x <? y)%Z (lookup d x l)
+        (ite (x >? y)%Z (lookup d x r) v)
+      ).
+  Proof. intros; exact eq_refl. Qed.
+
+  (** [insert k v t] is the map containing all the bindings of [t] along
+      with a binding of [k] to [v]. *)
+
+  Fixpoint insert (x : Z) (v : V) (t : tree) : tree :=
+    match t with
+    | Emp => Node Emp x v Emp
+    | Node l y v' r => 
+      ite (x <? y)%Z (Node (insert x v l) y v' r)
+      (ite (x >? y)%Z (Node l y v' (insert x v r))
+        (Node l x v r)
+      )
+    end.
+
+  Lemma insert_emp: 
+    forall x v, 
+      insert x v Emp = Node Emp x v Emp.
+  Proof. intros; exact eq_refl. Qed.
+
+  Lemma insert_node: 
+    forall x v l y v' r, 
+      insert x v (Node l y v' r) = ( 
+        ite (x <? y)%Z (Node (insert x v l) y v' r)
+        (ite (x >? y)%Z (Node l y v' (insert x v r))
+          (Node l x v r)
+        )
+      ).
+  Proof. intros; exact eq_refl. Qed.
+End Tree.
+
+Arguments Emp {_}.
+Arguments Node {_} _ _ _ _.
+Arguments bound {_} _ _.
+Arguments lookup {_} _ _ _.
+Arguments insert {_} _ _ _.
+
+Section FOLTree.
+
+  Variable (T: Type).
+
+  Inductive sorts : Set := | TS | TreeS | BS | ZS.
+
+  Scheme Equality for sorts.
+  Set Universe Polymorphism.
+
+  Inductive funs: arity sorts -> sorts -> Type :=
+    | b_lit : forall (b: bool), funs [] BS
+    | z_lt : funs [ZS; ZS] BS
+    | z_gt : funs [ZS; ZS] BS
+    | e_f : funs [] TreeS
+    | t_f : funs [TreeS; ZS; TS; TreeS] TreeS
+    | cond_b : funs [BS; BS; BS] BS
+    | cond_t : funs [BS; TS; TS] TS
+    | cond_tree : funs [BS; TreeS; TreeS] TreeS. 
+
+  Inductive rels: arity sorts -> Type :=.
+
+  Definition sig: signature :=
+    {| sig_sorts := sorts;
+      sig_funs := funs;
+      sig_rels := rels |}.
+
+  Definition fm ctx := FirstOrder.fm sig ctx.
+  Definition tm ctx := FirstOrder.tm sig ctx.
+
+  Definition mod_sorts (s: sig_sorts sig) : Type :=
+    match s with
+    | TreeS => tree T
+    | TS => T
+    | ZS => Z
+    | BS => bool
+    end.
+
+  Obligation Tactic := idtac.
+  Equations 
+    mod_fns params ret (f: sig_funs sig params ret) (args: HList.t mod_sorts params) 
+    : mod_sorts ret :=
+    { 
+      mod_fns _ _ (b_lit b) _ := b;
+      mod_fns _ _ z_lt (l ::: r ::: _) := (l <? r)%Z;
+      mod_fns _ _ z_gt (l ::: r ::: _) := (l >? r)%Z;
+      mod_fns _ _ e_f _ := Emp;
+      mod_fns _ _ t_f (l ::: k ::: v ::: r ::: _) := Node l k v r;
+      mod_fns _ _ cond_b (t ::: l ::: r ::: _) := ite t l r;
+      mod_fns _ _ cond_t (t ::: l ::: r ::: _) := ite t l r;
+      mod_fns _ _ cond_tree (t ::: l ::: r ::: _) := ite t l r;
+    }.
+
+  Definition mod_rels params
+    (args: sig_rels sig params)
+    (env: HList.t mod_sorts params) : Prop :=
+    match args with
+    end.
+
+  Program Definition fm_model : model sig := {|
+    FirstOrder.mod_sorts := mod_sorts;
+    FirstOrder.mod_fns := mod_fns;
+    FirstOrder.mod_rels := mod_rels;
+  |}.
+
+End FOLTree.
+
