src/theories/Reflection/Core.v
@@ -4,5 +4,111 @@ Require Export MetaCoq.Template.All.
 
 Require Import MetaCoq.Template.Checker.
 
-Definition eq_term (l r: term) : bool := 
-  @eq_term config.default_checker_flags init_graph l r.
+Fixpoint eq_term (l r: term) : bool := 
+  match l with
+  | tRel n =>
+    match r with
+    | tRel n' => PeanoNat.Nat.eqb n n'
+    | _ => false
+    end
+  | tVar id => 
+    match r with
+    | tVar id' => eq_string id id'
+    | _ => false
+    end
+  | tEvar ev args =>
+    match r with
+    | tEvar ev' args' => (PeanoNat.Nat.eqb ev ev' && forallb2 eq_term args args')%bool
+    | _ => false
+    end
+  | tSort _ =>
+    match r with
+    | tSort _ => true
+    | _ => false
+    end
+  | tCast f _ T =>
+    match r with
+    | tCast f' _ T' => (eq_term f f' && eq_term T T')%bool
+    | _ => false
+    end
+  | tProd _ b t0 =>
+    match r with
+    | tProd _ b' t' => (eq_term b b' && eq_term t0 t')%bool
+    | _ => false
+    end
+  | tLambda _ b t0 =>
+    match r with
+    | tLambda _ b' t' => (eq_term b b' && eq_term t0 t')%bool
+    | _ => false
+    end
+  | tLetIn _ b t0 c =>
+    match r with
+    | tLetIn _ b' t' c' => (eq_term b b' && eq_term t0 t' && eq_term c c')%bool
+    | _ => false
+    end
+  | tApp f args =>
+    match r with
+    | tApp f' args' => (eq_term f f' && forallb2 eq_term args args')%bool
+    | _ => false
+    end
+  | tConst c _ =>
+    match r with
+    | tConst c' _ => eq_constant c c'
+    | _ => false
+    end
+  | tInd i _ =>
+    match r with
+    | tInd i' _ => eq_inductive i i'
+    | _ => false
+    end
+  | tConstruct i k _ =>
+    match r with
+    | tConstruct i' k' _ => (eq_inductive i i' && PeanoNat.Nat.eqb k k')%bool
+    | _ => false
+    end
+  | tCase ind_nbparams_relevance p c brs =>
+    let (p0, _) := ind_nbparams_relevance in
+    let (ind, par) := p0 in
+      match r with
+      | tCase ind_nbparams_relevance0 p' c' brs' =>
+        let (p1, _) := ind_nbparams_relevance0 in
+        let (ind', par') := p1 in
+        (eq_inductive ind ind' && PeanoNat.Nat.eqb par par' &&
+          eq_term p p' && eq_term c c' &&
+          forallb2 (fun '(_, b) '(_, b') => eq_term b b') brs brs')%bool
+      | _ => false
+      end
+  | tProj p c =>
+    match r with
+    | tProj p' c' => (eq_projection p p' && eq_term c c')%bool
+    | _ => false
+    end
+  | tFix mfix idx =>
+    match r with
+    | tFix mfix' idx' =>
+      (forallb2
+          (fun x y : def term =>
+          eq_term (dtype x) (dtype y) &&
+          eq_term (dbody x) (dbody y)) mfix mfix' &&
+        PeanoNat.Nat.eqb idx idx')%bool
+    | _ => false
+    end
+  | tCoFix mfix idx =>
+    match r with
+    | tCoFix mfix' idx' =>
+      (forallb2
+          (fun x y : def term =>
+          eq_term (dtype x) (dtype y) &&
+          eq_term (dbody x) (dbody y)) mfix mfix' &&
+        PeanoNat.Nat.eqb idx idx')%bool
+    | _ => false
+    end
+  | _ => false
+  end.
+
+Definition eq_ctor (l r: term) : bool := 
+  match l, r with 
+  | tApp l' _, tApp r' _ => eq_term l' r'
+  | tApp l' _, _ => eq_term l' r
+  | _, _ => false
+  end.
