tests/vfa/SearchTree.v
@@ -1,0 +1,762 @@
+
+(** * SearchTree: Binary Search Trees *)
+(* Due to VFA's exercise on binary search trees: 
+  https://softwarefoundations.cis.upenn.edu/vfa-current/SearchTree.html
+*)
+
+Require Import MirrorSolve.FirstOrder.
+
+Require Import MirrorSolve.BV.
+Require Import MirrorSolve.SMT.
+Require Import MirrorSolve.UF.
+
+Require Import MirrorSolve.FOLTrees.
+
+Require Import MirrorSolve.HLists.
+Require Import Coq.Lists.List.
+
+Import HListNotations.
+Import ListNotations.
+
+Require Import Coq.Strings.String.
+
+Require Import MirrorSolve.Reflection.Core.
+Require Import MirrorSolve.Reflection.FM.
+
+From Hammer Require Import Hammer.
+
+Set Hammer ATPLimit 5.
+Set Hammer ReconstrLimit 10.
+
+Require Import Coq.ZArith.BinInt.
+
+Section Trees.
+  (* type of values in the tree *)
+  Variable (V: Type).
+  Set Universe Polymorphism.
+
+  (* UF symbols for trees: we model lookup, insert, and bound as UFs *)
+  
+  Notation sig := FOLTrees.sig.
+
+  Definition tree_model := FOLTrees.fm_model V.
+
+  Definition symbs : list (string * list (sig_sorts sig) * sig_sorts sig) := ([
+    ("lookup", [TS; ZS; TreeS], TS); 
+    ("insert", [ZS; TS; TreeS], TreeS); 
+    ("bound", [ZS; TreeS], BS) 
+  ]%string).
+
+  Lemma in_conv : forall {sym a r}, 
+    In (sym, a, r) symbs -> 
+    in_symbs sig sorts_eq_dec symbs sym a r = true.
+  Proof.
+    eapply UF.in_symbs_corr.
+  Defined.
+
+  Import HListNotations.
+
+  (* Interpretation function for UF symbols. 
+    In order for the reflection machinery to work out, we need to provide an actual interpretation for the UF symbols (even though they will be discharged as UF symbols in SMT).  *)
+  Definition interp_syms (sym: string) (a: list (sig_sorts sig)) (r: sig_sorts sig) (H: In (sym, a, r) symbs) (args: HList.t (FirstOrder.mod_sorts sig tree_model) a) : FirstOrder.mod_sorts sig tree_model r.
+    pose proof in_conv H.
+    unfold in_symbs in H0.
+    simpl in H0.
+    repeat match goal with 
+    | H: (if (?L =? ?R)%string then _ else _) = _ |- _ => 
+      destruct (comp_str_eqb_spec L R)
+    | H: (if ?A then _ else _) = _ |- _ => 
+      destruct A eqn:?
+    end; try congruence;
+    subst;
+    repeat match goal with 
+    | X: HList.t _ _ |- _ => 
+      inversion X; subst; clear X
+    end.
+    - exact (lookup X X1 X0).
+    - exact (insert X X1 X0).
+    - exact (bound X X1).
+  Defined.
+
+  Definition tree_uf_model := UF.fm_model sig tree_model symbs interp_syms.
+
+  Notation sig' := (UF.sig sig symbs).
+
+
+  Require Import MirrorSolve.Reflection.Core.
+  Require Import MirrorSolve.Reflection.FM.
+  Require Import MirrorSolve.Reflection.Tactics.
+
+  MetaCoq Quote Definition t_ite := @ite.
+  MetaCoq Quote Definition t_zlt := @Z.ltb.
+  MetaCoq Quote Definition t_glt := @Z.gtb.
+  MetaCoq Quote Definition t_emp := @Emp.
+  MetaCoq Quote Definition t_node := @Node.
+
+  MetaCoq Quote Definition t_insert := (@FOLTrees.insert V).
+  MetaCoq Quote Definition t_lookup := (@FOLTrees.lookup V).
+  MetaCoq Quote Definition t_bound := (@FOLTrees.bound V).
+
+  (* Some match tactics for the meta-interpreter. 
+    The meta-interpreter converts these definitions into a reflection procedure between pure Coq goals and FOL terms in the UF + Lists combined theory. 
+  *)
+
+  Definition is_emp t := eq_ctor t t_emp.
+  Definition is_node t := eq_ctor t t_node.
+  Definition is_zlt t := eq_term t t_zlt.
+  Definition is_zgt t := eq_term t t_glt.
+  Definition is_insert t := eq_ctor t t_insert.
+  Definition is_lookup t := eq_ctor t t_lookup.
+  Definition is_bound t := eq_ctor t t_bound.
+
+  MetaCoq Quote Definition t_bool := (bool).
+  MetaCoq Quote Definition t_Z := (Z).
+  MetaCoq Quote Definition t_tree := (@tree V).
+  MetaCoq Quote Definition t_V := (V).
+
+  Definition is_cond_b t :=
+    match t with 
+    | tApp f (t :: _) => 
+      andb (eq_term f t_ite) (eq_term t t_bool)
+    | _ => false
+    end.
+
+  Definition is_cond_t t :=
+    match t with 
+    | tApp f (t :: _) => 
+      andb (eq_term f t_ite) (eq_term t t_V)
+    | _ => false
+    end.
+
+  Definition is_cond_tree t :=
+    match t with 
+    | tApp f (t :: _) => 
+      andb (eq_term f t_ite) (eq_term t t_tree)
+    | _ => false
+    end.
+
+  Notation blit := (tacLit sig' tree_uf_model bool_lit).
+
+  Definition match_tacs : list ((term -> bool) * tac_syn sig' tree_uf_model) := [
+      ( is_emp, tacFun _ _ (Mk_fun_sym sig' _ _ (CFun _ symbs e_f)))
+    ; ( is_node, tacFun _ _ (Mk_fun_sym sig' _ _ (CFun _ symbs t_f)))
+    ; ( is_zlt, tacFun _ _ (Mk_fun_sym sig' _ _ (CFun _ symbs z_lt)))
+    ; ( is_zgt, tacFun _ _ (Mk_fun_sym sig' _ _ (CFun _ symbs z_gt)))
+    ; ( is_cond_b, tacFun _ _ (Mk_fun_sym sig' _ _ (CFun _ symbs cond_b)))
+    ; ( is_cond_t, tacFun _ _ (Mk_fun_sym sig' _ _ (CFun _ symbs cond_t)))
+    ; ( is_cond_tree, tacFun _ _ (Mk_fun_sym sig' _ _ (CFun _ symbs cond_tree)))
+    ; ( is_bool_term, blit 
+        (fun b => existT _ BS b) 
+        (fun b _ => existT _ BS (TFun sig' (CFun _ symbs (b_lit b)) hnil)))
+    ; ( is_lookup, tacFun _ _ (Mk_fun_sym sig' _ _ (UFun (s := "lookup") _ symbs ltac:(solve_uf_membership))))
+    ; ( is_bound, tacFun _ _ (Mk_fun_sym sig' _ _ (UFun (s := "bound") _ symbs ltac:(solve_uf_membership))))
+    ; ( is_insert, tacFun _ _ (Mk_fun_sym sig' _ _ (UFun (s := "insert") _ symbs ltac:(solve_uf_membership))))
+  ].
+
+  (* This is an analogous match but for reflecting Coq types into FOL sorts. *)
+  Definition match_inds : list ((term -> bool) * FOLTrees.sorts) := [
+      (eq_term t_tree, TreeS)
+    ; (eq_term t_V, TS)
+    ; (eq_term t_bool, BS)
+    ; (eq_term t_Z, ZS)
+  ].
+
+  Local Declare ML Module "mirrorsolve".
+  RegisterCustomSort TS "A".
+
+  RegisterSMTInd TreeS (SICases [
+    ("node"%string, [SIRec; SISort (SInt tt); SISort (SCustom "A"); SIRec]); 
+    ("emp"%string, [])
+    ]) "A_tree".
+
+  RegisterSMTSort ZS SInt.
+  RegisterSMTSort BS SBool.
+
+  (* first argument is the return type, the rest are the argument types *)
+  RegisterSMTUF "bound" BS ZS TreeS.
+  RegisterSMTUF "lookup" TS TS ZS TreeS.
+  RegisterSMTUF "insert" TreeS ZS TS TreeS.
+
+  Transparent denote_tm.
+
+  RegisterSMTFun FOLTrees.z_lt "<" 2.
+  RegisterSMTFun FOLTrees.z_gt ">" 2.
+  RegisterSMTFun FOLTrees.e_f "emp" 0.
+  RegisterSMTFun FOLTrees.t_f "node" 4.
+  RegisterSMTFun FOLTrees.cond_b "ite" 3.
+  RegisterSMTFun FOLTrees.cond_t "ite" 3.
+  RegisterSMTFun FOLTrees.cond_tree "ite" 3.
+
+  RegisterSMTBuiltin FOLTrees.b_lit BoolLit.
+
+  Require Import MirrorSolve.Axioms.
+
+  Ltac check_goal_sat := 
+    match goal with 
+    | |- ?G => check_interp_pos G; eapply UnsoundAxioms.interp_true
+    end.
+  Ltac check_goal_unsat := 
+    match goal with 
+    | |- ?G => check_unsat_neg G; eapply UnsoundAxioms.interp_true
+    end.
+
+  Locate pose_all.
+
+  Ltac pose_lookup_axioms := Utils.pose_all (tt, @lookup_emp V, @lookup_node V).
+  Ltac pose_bound_axioms := Utils.pose_all (tt, @bound_emp V, @bound_node V).
+  Ltac pose_insert_axioms := Utils.pose_all (tt, @insert_emp V, @insert_node V).
+
+  Ltac pose_tree_axioms := pose_lookup_axioms; pose_bound_axioms; pose_insert_axioms.
+
+  Ltac prep_proof := pose_tree_axioms; Utils.revert_all; intros ?.
+
+(* ################################################################# *)
+(** * Correctness of BST Operations *)
+
+(** To prove the correctness of [lookup] and [bound], we need
+    specifications for them.  We'll study two different techniques for
+    that in this chapter. *)
+
+(** The first is called _algebraic specification_.  With it, we write
+    down equations relating the results of operations.  For example,
+    we could write down equations like the following to specify the
+    [+] and [*] operations:
+
+      (a + b) + c = a + (b + c)
+      a + b = b + a
+      a + 0 = a
+      (a * b) * c = a * (b * c)
+      a * b = b * a
+      a * 1 = a
+      a * 0 = 0
+      a * (b + c) = a * b + a * c
+
+    For BSTs, let's examine how [lookup] should interact with
+    when applied to other operations.  It is easy to see what needs to
+    be true for [empty_tree]: looking up any value at all in the empty
+    tree should fail and return the default value:
+
+      lookup d k empty_tree = d
+
+    What about non-empty trees?  The only way to build a non-empty
+    tree is by applying [insert k v t] to an existing tree [t]. So it
+    suffices to describe the behavior of [lookup] on the result of an
+    arbitrary [insert] operation. There are two cases.  If we look up
+    the same key that was just inserted, we should get the value that
+    was inserted with it:
+
+      lookup d k (insert k v t) = v
+
+    If we look up a different key than was just inserted, the insert
+    should not affect the answer -- which should be the same as if we
+    did the lookup in the original tree before the insert occured:
+
+      lookup d k' (insert k v t) = lookup d k' t      if k <> k'
+
+    These three basic equations specify the correct behavior of maps.
+    Let's prove that they hold. *)
+  MetaCoq Quote Definition lookup_empty_goal := (
+    (forall (d : V) (x : Z) (l : tree V) (y : Z) 
+    (v : V) (r : tree V),
+  lookup d x (Node l y v r) =
+  ite (x <? y)%Z (lookup d x l)
+    (ite (x >? y)%Z (lookup d x r) v)) ->
+ (forall (d : V) (x : Z), lookup d x Emp = d) ->
+ (forall (x : Z) (l : tree V) (y : Z) (v : V) (r : tree V),
+  bound x (Node l y v r) =
+  ite (x <? y)%Z (bound x l)
+    (ite (x >? y)%Z (bound x r) true)) ->
+ (forall x : Z, bound x Emp = false) ->
+ (forall (x : Z) (v : V) (l : tree V) (y : Z) 
+    (v' : V) (r : tree V),
+  insert x v (Node l y v' r) =
+  ite (x <? y)%Z (Node (insert x v l) y v' r)
+    (ite (x >? y)%Z (Node l y v' (insert x v r))
+       (Node l x v r))) ->
+ (forall (x : Z) (v : V), insert x v Emp = Node Emp x v Emp) ->
+ forall (d : V) (k : Z), lookup d k Emp = d
+  ).
+
+  (* MetaCoq Quote Definition  *)
+
+  (* hammer handles this one (it's easy) *)
+  SetSMTSolver "cvc5".
+  Theorem lookup_empty : 
+    forall (d: V) (k : Z),
+      lookup d k Emp = d.
+  Proof.
+    prep_proof.
+    reflect_goal (UF.sig sig symbs) tree_uf_model sorts_eq_dec match_tacs match_inds lookup_empty_goal. 
+    check_goal_unsat.
+  Admitted. (* some weird evaluation issue, can't QED... *)
+
+
+  MetaCoq Quote Definition lookup_insert_emp := (
+    (forall (d : V) (x : Z) (l : tree V) (y : Z) (v : V) (r : tree V),
+    lookup d x (Node l y v r) =
+    ite (x <? y)%Z (lookup d x l) (ite (x >? y)%Z (lookup d x r) v)) ->
+   (forall (d : V) (x : Z), lookup d x Emp = d) ->
+   (forall (x : Z) (l : tree V) (y : Z) (v : V) (r : tree V),
+    bound x (Node l y v r) =
+    ite (x <? y)%Z (bound x l) (ite (x >? y)%Z (bound x r) true)) ->
+   (forall x : Z, bound x Emp = false) ->
+   (forall (x : Z) (v : V) (l : tree V) (y : Z) (v' : V) (r : tree V),
+    insert x v (Node l y v' r) =
+    ite (x <? y)%Z (Node (insert x v l) y v' r)
+      (ite (x >? y)%Z (Node l y v' (insert x v r)) (Node l x v r))) ->
+   (forall (x : Z) (v : V), insert x v Emp = Node Emp x v Emp) ->
+   forall (d : V) (k : Z) (v : V), lookup d k (insert k v Emp) = v
+  ).
+
+  MetaCoq Quote Definition lookup_insert_node := (
+    forall (t1 : tree V) (k : Z) (v : V) (t2 : tree V),
+    (forall (d : V) (k0 : Z) (v0 : V), lookup d k0 (insert k0 v0 t1) = v0) ->
+    (forall (d : V) (k0 : Z) (v0 : V), lookup d k0 (insert k0 v0 t2) = v0) ->
+    (forall (d : V) (x : Z) (l : tree V) (y : Z) (v0 : V) (r : tree V),
+     lookup d x (Node l y v0 r) =
+     ite (x <? y)%Z (lookup d x l) (ite (x >? y)%Z (lookup d x r) v0)) ->
+    (forall (d : V) (x : Z), lookup d x Emp = d) ->
+    (forall (x : Z) (l : tree V) (y : Z) (v0 : V) (r : tree V),
+     bound x (Node l y v0 r) =
+     ite (x <? y)%Z (bound x l) (ite (x >? y)%Z (bound x r) true)) ->
+    (forall x : Z, bound x Emp = false) ->
+    (forall (x : Z) (v0 : V) (l : tree V) (y : Z) (v' : V) (r : tree V),
+     insert x v0 (Node l y v' r) =
+     ite (x <? y)%Z (Node (insert x v0 l) y v' r)
+       (ite (x >? y)%Z (Node l y v' (insert x v0 r)) (Node l x v0 r))) ->
+    (forall (x : Z) (v0 : V), insert x v0 Emp = Node Emp x v0 Emp) ->
+    forall (d : V) (k0 : Z) (v0 : V),
+    lookup d k0 (insert k0 v0 (Node t1 k v t2)) = v0
+  ).
+
+
+  (* hammer handles this one *)
+  Theorem lookup_insert_eq : 
+    forall (t : tree V) d k v,
+      lookup d k (insert k v t)  = v.
+  Proof.
+    induction t; prep_proof.
+    - reflect_goal (UF.sig sig symbs) tree_uf_model sorts_eq_dec match_tacs match_inds lookup_insert_emp. 
+      check_goal_unsat.
+    - reflect_goal (UF.sig sig symbs) tree_uf_model sorts_eq_dec match_tacs match_inds lookup_insert_node. 
+      check_goal_unsat.
+  Admitted.
+
+
+  MetaCoq Quote Definition lookup_insert_neq_emp := (
+    (forall (d : V) (x : Z) (l : tree V) (y : Z) (v : V) (r : tree V),
+ lookup d x (Node l y v r) =
+ ite (x <? y)%Z (lookup d x l) (ite (x >? y)%Z (lookup d x r) v)) ->
+(forall (d : V) (x : Z), lookup d x Emp = d) ->
+(forall (x : Z) (l : tree V) (y : Z) (v : V) (r : tree V),
+ bound x (Node l y v r) =
+ ite (x <? y)%Z (bound x l) (ite (x >? y)%Z (bound x r) true)) ->
+(forall x : Z, bound x Emp = false) ->
+(forall (x : Z) (v : V) (l : tree V) (y : Z) (v' : V) (r : tree V),
+ insert x v (Node l y v' r) =
+ ite (x <? y)%Z (Node (insert x v l) y v' r)
+   (ite (x >? y)%Z (Node l y v' (insert x v r)) (Node l x v r))) ->
+(forall (x : Z) (v : V), insert x v Emp = Node Emp x v Emp) ->
+forall (d : V) (k k' : Z) (v : V),
+k <> k' -> lookup d k' (insert k v Emp) = lookup d k' Emp
+  ).
+
+
+  MetaCoq Quote Definition lookup_insert_neq_node := (
+    forall (t1 : tree V) (k : Z) (v : V) (t2 : tree V),
+    (forall (d : V) (k0 k' : Z) (v0 : V),
+     k0 <> k' -> lookup d k' (insert k0 v0 t1) = lookup d k' t1) ->
+    (forall (d : V) (k0 k' : Z) (v0 : V),
+     k0 <> k' -> lookup d k' (insert k0 v0 t2) = lookup d k' t2) ->
+    (forall (d : V) (x : Z) (l : tree V) (y : Z) (v0 : V) (r : tree V),
+     lookup d x (Node l y v0 r) =
+     ite (x <? y)%Z (lookup d x l) (ite (x >? y)%Z (lookup d x r) v0)) ->
+    (forall (d : V) (x : Z), lookup d x Emp = d) ->
+    (forall (x : Z) (l : tree V) (y : Z) (v0 : V) (r : tree V),
+     bound x (Node l y v0 r) =
+     ite (x <? y)%Z (bound x l) (ite (x >? y)%Z (bound x r) true)) ->
+    (forall x : Z, bound x Emp = false) ->
+    (forall (x : Z) (v0 : V) (l : tree V) (y : Z) (v' : V) (r : tree V),
+     insert x v0 (Node l y v' r) =
+     ite (x <? y)%Z (Node (insert x v0 l) y v' r)
+       (ite (x >? y)%Z (Node l y v' (insert x v0 r)) (Node l x v0 r))) ->
+    (forall (x : Z) (v0 : V), insert x v0 Emp = Node Emp x v0 Emp) ->
+    forall (d : V) (k0 k' : Z) (v0 : V),
+    k0 <> k' ->
+    lookup d k' (insert k0 v0 (Node t1 k v t2)) = lookup d k' (Node t1 k v t2)
+  ).
+
+
+  (* hammer does not handle this one *)
+  Theorem lookup_insert_neq :
+    forall (t: tree V) d k k' v,
+      k <> k' -> 
+      lookup d k' (insert k v t) = lookup d k' t.
+  Proof.
+    induction t; prep_proof.
+    - 
+      reflect_goal (UF.sig sig symbs) tree_uf_model sorts_eq_dec match_tacs match_inds lookup_insert_neq_emp. 
+      check_goal_unsat.
+    - 
+      reflect_goal (UF.sig sig symbs) tree_uf_model sorts_eq_dec match_tacs match_inds lookup_insert_neq_node. 
+      check_goal_unsat.
+  Admitted.
+
+(** **** Exercise: 3 stars, standard, optional (bound_correct) *)
+
+(** Specify and prove the correctness of [bound]. State and prove
+    three theorems, inspired by those we just proved for [lookup]. *)
+
+(* FILL IN HERE *)
+
+(** **** Exercise: 3 stars, standard, optional (bound_default) *)
+
+(** Prove that if [bound] returns [false], then [lookup] returns
+    the default value. Proceed by induction on the tree. *)
+
+
+    MetaCoq Quote Definition bound_default_emp := (
+      forall (k : Z) (d : V),
+      (forall (d0 : V) (x : Z) (l : tree V) (y : Z) (v : V) (r : tree V),
+       lookup d0 x (Node l y v r) =
+       ite (x <? y)%Z (lookup d0 x l) (ite (x >? y)%Z (lookup d0 x r) v)) ->
+      (forall (d0 : V) (x : Z), lookup d0 x Emp = d0) ->
+      (forall (x : Z) (l : tree V) (y : Z) (v : V) (r : tree V),
+       bound x (Node l y v r) =
+       ite (x <? y)%Z (bound x l) (ite (x >? y)%Z (bound x r) true)) ->
+      (forall x : Z, bound x Emp = false) ->
+      (forall (x : Z) (v : V) (l : tree V) (y : Z) (v' : V) (r : tree V),
+       insert x v (Node l y v' r) =
+       ite (x <? y)%Z (Node (insert x v l) y v' r)
+         (ite (x >? y)%Z (Node l y v' (insert x v r)) (Node l x v r))) ->
+      (forall (x : Z) (v : V), insert x v Emp = Node Emp x v Emp) ->
+      bound k Emp = false -> lookup d k Emp = d
+    ).
+  
+  
+    MetaCoq Quote Definition bound_default_node := (
+      forall (k : Z) (d : V) (t1 : tree V) (k0 : Z) (v : V) (t2 : tree V),
+      (bound k t1 = false -> lookup d k t1 = d) ->
+      (bound k t2 = false -> lookup d k t2 = d) ->
+      (forall (d0 : V) (x : Z) (l : tree V) (y : Z) (v0 : V) (r : tree V),
+       lookup d0 x (Node l y v0 r) =
+       ite (x <? y)%Z (lookup d0 x l) (ite (x >? y)%Z (lookup d0 x r) v0)) ->
+      (forall (d0 : V) (x : Z), lookup d0 x Emp = d0) ->
+      (forall (x : Z) (l : tree V) (y : Z) (v0 : V) (r : tree V),
+       bound x (Node l y v0 r) =
+       ite (x <? y)%Z (bound x l) (ite (x >? y)%Z (bound x r) true)) ->
+      (forall x : Z, bound x Emp = false) ->
+      (forall (x : Z) (v0 : V) (l : tree V) (y : Z) (v' : V) (r : tree V),
+       insert x v0 (Node l y v' r) =
+       ite (x <? y)%Z (Node (insert x v0 l) y v' r)
+         (ite (x >? y)%Z (Node l y v' (insert x v0 r)) (Node l x v0 r))) ->
+      (forall (x : Z) (v0 : V), insert x v0 Emp = Node Emp x v0 Emp) ->
+      bound k (Node t1 k0 v t2) = false -> lookup d k (Node t1 k0 v t2) = d
+    ).
+
+    (* hammer handles this one *)
+  Theorem bound_default :
+    forall k d (t: tree V),
+      bound k t = false ->
+      lookup d k t = d.
+  Proof.
+    induction t; prep_proof. 
+
+    - reflect_goal (UF.sig sig symbs) tree_uf_model sorts_eq_dec match_tacs match_inds bound_default_emp. 
+      check_goal_unsat.
+    - reflect_goal (UF.sig sig symbs) tree_uf_model sorts_eq_dec match_tacs match_inds bound_default_node. 
+      check_goal_unsat.
+  Admitted.
+
+(** [] *)
+
+(* ################################################################# *)
+(** * BSTs vs. Higher-order Functions (Optional) *)
+
+(** The three theorems we just proved for [lookup] should seem
+    familiar: we proved equivalent theorems in [Maps] for maps
+    defined as higher-order functions. *)
+
+(** Let's prove analogues to these three theorems for search trees.
+
+    Hint: you do not need to unfold the definitions of [empty_tree],
+    [insert], or [lookup].  Instead, use [lookup_insert_eq] and
+    [lookup_insert_neq]. *)
+
+(** **** Exercise: 2 stars, standard, optional (lookup_insert_shadow) *)
+
+
+
+MetaCoq Quote Definition lookup_insert_shadow_emp := (
+  (forall (d : V) (x : Z) (l : tree V) (y : Z) (v : V) (r : tree V),
+ lookup d x (Node l y v r) =
+ ite (x <? y)%Z (lookup d x l) (ite (x >? y)%Z (lookup d x r) v)) ->
+(forall (d : V) (x : Z), lookup d x Emp = d) ->
+(forall (x : Z) (l : tree V) (y : Z) (v : V) (r : tree V),
+ bound x (Node l y v r) =
+ ite (x <? y)%Z (bound x l) (ite (x >? y)%Z (bound x r) true)) ->
+(forall x : Z, bound x Emp = false) ->
+(forall (x : Z) (v : V) (l : tree V) (y : Z) (v' : V) (r : tree V),
+ insert x v (Node l y v' r) =
+ ite (x <? y)%Z (Node (insert x v l) y v' r)
+   (ite (x >? y)%Z (Node l y v' (insert x v r)) (Node l x v r))) ->
+(forall (x : Z) (v : V), insert x v Emp = Node Emp x v Emp) ->
+forall (v v' d : V) (k k' : Z),
+lookup d k' (insert k v (insert k v' Emp)) = lookup d k' (insert k v Emp)
+).
+
+
+MetaCoq Quote Definition lookup_insert_shadow_node := (
+  forall (t1 : tree V) (k : Z) (v : V) (t2 : tree V),
+(forall (v0 v' d : V) (k0 k' : Z),
+ lookup d k' (insert k0 v0 (insert k0 v' t1)) = lookup d k' (insert k0 v0 t1)) ->
+(forall (v0 v' d : V) (k0 k' : Z),
+ lookup d k' (insert k0 v0 (insert k0 v' t2)) = lookup d k' (insert k0 v0 t2)) ->
+(forall (d : V) (x : Z) (l : tree V) (y : Z) (v0 : V) (r : tree V),
+ lookup d x (Node l y v0 r) =
+ ite (x <? y)%Z (lookup d x l) (ite (x >? y)%Z (lookup d x r) v0)) ->
+(forall (d : V) (x : Z), lookup d x Emp = d) ->
+(forall (x : Z) (l : tree V) (y : Z) (v0 : V) (r : tree V),
+ bound x (Node l y v0 r) =
+ ite (x <? y)%Z (bound x l) (ite (x >? y)%Z (bound x r) true)) ->
+(forall x : Z, bound x Emp = false) ->
+(forall (x : Z) (v0 : V) (l : tree V) (y : Z) (v' : V) (r : tree V),
+ insert x v0 (Node l y v' r) =
+ ite (x <? y)%Z (Node (insert x v0 l) y v' r)
+   (ite (x >? y)%Z (Node l y v' (insert x v0 r)) (Node l x v0 r))) ->
+(forall (x : Z) (v0 : V), insert x v0 Emp = Node Emp x v0 Emp) ->
+forall (v0 v' d : V) (k0 k' : Z),
+lookup d k' (insert k0 v0 (insert k0 v' (Node t1 k v t2))) =
+lookup d k' (insert k0 v0 (Node t1 k v t2))
+).
+
+  (* hammer does not handle this one *)
+  Lemma lookup_insert_shadow :
+    forall (t: tree V) v v' d k k',
+      lookup d k' (insert k v (insert k v' t)) = lookup d k' (insert k v t).
+  Proof. 
+    induction t; prep_proof.
+
+    - reflect_goal (UF.sig sig symbs) tree_uf_model sorts_eq_dec match_tacs match_inds lookup_insert_shadow_emp. 
+      check_goal_unsat.
+    - reflect_goal (UF.sig sig symbs) tree_uf_model sorts_eq_dec match_tacs match_inds lookup_insert_shadow_node. 
+      check_goal_unsat.
+  Admitted.
+
+
+  MetaCoq Quote Definition lookup_insert_same_emp := (
+    forall (k k' : Z) (d : V),
+(forall (d0 : V) (x : Z) (l : tree V) (y : Z) (v : V) (r : tree V),
+ lookup d0 x (Node l y v r) =
+ ite (x <? y)%Z (lookup d0 x l) (ite (x >? y)%Z (lookup d0 x r) v)) ->
+(forall (d0 : V) (x : Z), lookup d0 x Emp = d0) ->
+(forall (x : Z) (l : tree V) (y : Z) (v : V) (r : tree V),
+ bound x (Node l y v r) =
+ ite (x <? y)%Z (bound x l) (ite (x >? y)%Z (bound x r) true)) ->
+(forall x : Z, bound x Emp = false) ->
+(forall (x : Z) (v : V) (l : tree V) (y : Z) (v' : V) (r : tree V),
+ insert x v (Node l y v' r) =
+ ite (x <? y)%Z (Node (insert x v l) y v' r)
+   (ite (x >? y)%Z (Node l y v' (insert x v r)) (Node l x v r))) ->
+(forall (x : Z) (v : V), insert x v Emp = Node Emp x v Emp) ->
+lookup d k' (insert k (lookup d k Emp) Emp) = lookup d k' Emp
+  ).
+  
+  
+  MetaCoq Quote Definition lookup_insert_same_node := (
+    forall (k k' : Z) (d : V) (t1 : tree V) (k0 : Z) (v : V) (t2 : tree V),
+lookup d k' (insert k (lookup d k t1) t1) = lookup d k' t1 ->
+lookup d k' (insert k (lookup d k t2) t2) = lookup d k' t2 ->
+(forall (d0 : V) (x : Z) (l : tree V) (y : Z) (v0 : V) (r : tree V),
+ lookup d0 x (Node l y v0 r) =
+ ite (x <? y)%Z (lookup d0 x l) (ite (x >? y)%Z (lookup d0 x r) v0)) ->
+(forall (d0 : V) (x : Z), lookup d0 x Emp = d0) ->
+(forall (x : Z) (l : tree V) (y : Z) (v0 : V) (r : tree V),
+ bound x (Node l y v0 r) =
+ ite (x <? y)%Z (bound x l) (ite (x >? y)%Z (bound x r) true)) ->
+(forall x : Z, bound x Emp = false) ->
+(forall (x : Z) (v0 : V) (l : tree V) (y : Z) (v' : V) (r : tree V),
+ insert x v0 (Node l y v' r) =
+ ite (x <? y)%Z (Node (insert x v0 l) y v' r)
+   (ite (x >? y)%Z (Node l y v' (insert x v0 r)) (Node l x v0 r))) ->
+(forall (x : Z) (v0 : V), insert x v0 Emp = Node Emp x v0 Emp) ->
+lookup d k' (insert k (lookup d k (Node t1 k0 v t2)) (Node t1 k0 v t2)) =
+lookup d k' (Node t1 k0 v t2)
+  ).
+
+  (** **** Exercise: 2 stars, standard, optional (lookup_insert_same) *)
+
+  (* hammer does not handle this one *)
+  Lemma lookup_insert_same :
+    forall k k' d (t: tree V),
+      lookup d k' (insert k (lookup d k t) t) = lookup d k' t.
+  Proof. 
+    induction t; prep_proof.
+
+    - reflect_goal (UF.sig sig symbs) tree_uf_model sorts_eq_dec match_tacs match_inds lookup_insert_same_emp. 
+      check_goal_unsat.
+    - reflect_goal (UF.sig sig symbs) tree_uf_model sorts_eq_dec match_tacs match_inds lookup_insert_same_node. 
+      check_goal_unsat.
+  Admitted.
+
+
+
+  MetaCoq Quote Definition lookup_insert_permute_emp := (
+    forall (v1 v2 d : V) (k1 k2 k' : Z),
+(forall (d0 : V) (x : Z) (l : tree V) (y : Z) (v : V) (r : tree V),
+ lookup d0 x (Node l y v r) =
+ ite (x <? y)%Z (lookup d0 x l) (ite (x >? y)%Z (lookup d0 x r) v)) ->
+(forall (d0 : V) (x : Z), lookup d0 x Emp = d0) ->
+(forall (x : Z) (l : tree V) (y : Z) (v : V) (r : tree V),
+ bound x (Node l y v r) =
+ ite (x <? y)%Z (bound x l) (ite (x >? y)%Z (bound x r) true)) ->
+(forall x : Z, bound x Emp = false) ->
+(forall (x : Z) (v : V) (l : tree V) (y : Z) (v' : V) (r : tree V),
+ insert x v (Node l y v' r) =
+ ite (x <? y)%Z (Node (insert x v l) y v' r)
+   (ite (x >? y)%Z (Node l y v' (insert x v r)) (Node l x v r))) ->
+(forall (x : Z) (v : V), insert x v Emp = Node Emp x v Emp) ->
+k1 <> k2 ->
+lookup d k' (insert k1 v1 (insert k2 v2 Emp)) =
+lookup d k' (insert k2 v2 (insert k1 v1 Emp))
+).
+  
+  
+  MetaCoq Quote Definition lookup_insert_permute_node := (
+    forall (v1 v2 d : V) (k1 k2 k' : Z) (t1 : tree V) 
+    (k : Z) (v : V) (t2 : tree V),
+  (k1 <> k2 ->
+   lookup d k' (insert k1 v1 (insert k2 v2 t1)) =
+   lookup d k' (insert k2 v2 (insert k1 v1 t1))) ->
+  (k1 <> k2 ->
+   lookup d k' (insert k1 v1 (insert k2 v2 t2)) =
+   lookup d k' (insert k2 v2 (insert k1 v1 t2))) ->
+  (forall (d0 : V) (x : Z) (l : tree V) (y : Z) (v0 : V) (r : tree V),
+   lookup d0 x (Node l y v0 r) =
+   ite (x <? y)%Z (lookup d0 x l) (ite (x >? y)%Z (lookup d0 x r) v0)) ->
+  (forall (d0 : V) (x : Z), lookup d0 x Emp = d0) ->
+  (forall (x : Z) (l : tree V) (y : Z) (v0 : V) (r : tree V),
+   bound x (Node l y v0 r) =
+   ite (x <? y)%Z (bound x l) (ite (x >? y)%Z (bound x r) true)) ->
+  (forall x : Z, bound x Emp = false) ->
+  (forall (x : Z) (v0 : V) (l : tree V) (y : Z) (v' : V) (r : tree V),
+   insert x v0 (Node l y v' r) =
+   ite (x <? y)%Z (Node (insert x v0 l) y v' r)
+     (ite (x >? y)%Z (Node l y v' (insert x v0 r)) (Node l x v0 r))) ->
+  (forall (x : Z) (v0 : V), insert x v0 Emp = Node Emp x v0 Emp) ->
+  k1 <> k2 ->
+  lookup d k' (insert k1 v1 (insert k2 v2 (Node t1 k v t2))) =
+  lookup d k' (insert k2 v2 (insert k1 v1 (Node t1 k v t2)))
+  ).
+
+  (** **** Exercise: 2 stars, standard, optional (lookup_insert_permute) *)
+
+  (* hammer does not handle this one *)
+  Lemma lookup_insert_permute :
+    forall v1 v2 d k1 k2 k' (t: tree V),
+      k1 <> k2 ->
+      lookup d k' (insert k1 v1 (insert k2 v2 t))
+      = lookup d k' (insert k2 v2 (insert k1 v1 t)).
+  Proof. 
+    induction t; prep_proof.
+
+    - reflect_goal (UF.sig sig symbs) tree_uf_model sorts_eq_dec match_tacs match_inds lookup_insert_permute_emp. 
+      check_goal_unsat.
+    - reflect_goal (UF.sig sig symbs) tree_uf_model sorts_eq_dec match_tacs match_inds lookup_insert_permute_node. 
+      check_goal_unsat.
+
+  Admitted.
+
+(** Our ability to prove these lemmas without reference to the
+    underlying tree implementation demonstrates they hold for any map
+    implementation that satisfies the three basic equations. *)
+
+(** Each of these lemmas just proved was phrased as an equality
+    between the results of looking up an arbitrary key [k'] in two
+    maps.  But the lemmas for the function-based maps were phrased as
+    direct equalities between the maps themselves.
+
+    Could we state the tree lemmas with direct equalities?  For
+    [insert_shadow], the answer is yes: *)
+
+
+    MetaCoq Quote Definition insert_shadow_equality_emp := (
+      (forall (d : V) (x : Z) (l : tree V) (y : Z) (v : V) (r : tree V),
+      lookup d x (Node l y v r) =
+      ite (x <? y)%Z (lookup d x l) (ite (x >? y)%Z (lookup d x r) v)) ->
+     (forall (d : V) (x : Z), lookup d x Emp = d) ->
+     (forall (x : Z) (l : tree V) (y : Z) (v : V) (r : tree V),
+      bound x (Node l y v r) =
+      ite (x <? y)%Z (bound x l) (ite (x >? y)%Z (bound x r) true)) ->
+     (forall x : Z, bound x Emp = false) ->
+     (forall (x : Z) (v : V) (l : tree V) (y : Z) (v' : V) (r : tree V),
+      insert x v (Node l y v' r) =
+      ite (x <? y)%Z (Node (insert x v l) y v' r)
+        (ite (x >? y)%Z (Node l y v' (insert x v r)) (Node l x v r))) ->
+     (forall (x : Z) (v : V), insert x v Emp = Node Emp x v Emp) ->
+     forall (k : Z) (v v' : V), insert k v (insert k v' Emp) = insert k v Emp
+  ).
+    
+    
+    MetaCoq Quote Definition insert_shadow_equality_node := (
+      forall (t1 : tree V) (k : Z) (v : V) (t2 : tree V),
+      (forall (k0 : Z) (v0 v' : V),
+       insert k0 v0 (insert k0 v' t1) = insert k0 v0 t1) ->
+      (forall (k0 : Z) (v0 v' : V),
+       insert k0 v0 (insert k0 v' t2) = insert k0 v0 t2) ->
+      (forall (d : V) (x : Z) (l : tree V) (y : Z) (v0 : V) (r : tree V),
+       lookup d x (Node l y v0 r) =
+       ite (x <? y)%Z (lookup d x l) (ite (x >? y)%Z (lookup d x r) v0)) ->
+      (forall (d : V) (x : Z), lookup d x Emp = d) ->
+      (forall (x : Z) (l : tree V) (y : Z) (v0 : V) (r : tree V),
+       bound x (Node l y v0 r) =
+       ite (x <? y)%Z (bound x l) (ite (x >? y)%Z (bound x r) true)) ->
+      (forall x : Z, bound x Emp = false) ->
+      (forall (x : Z) (v0 : V) (l : tree V) (y : Z) (v' : V) (r : tree V),
+       insert x v0 (Node l y v' r) =
+       ite (x <? y)%Z (Node (insert x v0 l) y v' r)
+         (ite (x >? y)%Z (Node l y v' (insert x v0 r)) (Node l x v0 r))) ->
+      (forall (x : Z) (v0 : V), insert x v0 Emp = Node Emp x v0 Emp) ->
+      forall (k0 : Z) (v0 v' : V),
+      insert k0 v0 (insert k0 v' (Node t1 k v t2)) = insert k0 v0 (Node t1 k v t2)
+    ).
+
+
+
+  (* hammer does not handle this one *)
+  Lemma insert_shadow_equality : 
+    forall (t: tree V) k v v',
+      insert k v (insert k v' t) = insert k v t.
+  Proof.
+    induction t; prep_proof.
+
+    - reflect_goal (UF.sig sig symbs) tree_uf_model sorts_eq_dec match_tacs match_inds insert_shadow_equality_emp. 
+      check_goal_unsat.
+    - reflect_goal (UF.sig sig symbs) tree_uf_model sorts_eq_dec match_tacs match_inds insert_shadow_equality_node. 
+      check_goal_unsat.
+  Admitted.
+
+(** But the other two direct equalities on BSTs do not necessarily
+    hold. *)
+
+(** **** Exercise: 3 stars, standard, optional (direct_equalities_break) *)
+
+(** Prove that the other equalities do not hold.  Hint: find a counterexample
+    first on paper, then use the [exists] tactic to instantiate the theorem
+    on your counterexample.  The simpler your counterexample, the simpler
+    the rest of the proof will be. *)
+
+(* Lemma insert_same_equality_breaks :
+  exists (V : Type) (d : V) (t : tree V) (k : key),
+      insert k (lookup d k t) t <> t.
+Proof.
+  (* FILL IN HERE *) Admitted.
+
+Lemma insert_permute_equality_breaks :
+  exists (V : Type) (v1 v2 : V) (k1 k2 : key) (t : tree V),
+    k1 <> k2 /\ insert k1 v1 (insert k2 v2 t) <> insert k2 v2 (insert k1 v1 t).
+Proof.
+  (* FILL IN HERE *) Admitted. *)
+
+(** [] *)
+
